aes/verif_setkey_enc_LL.v
@@ -70,114 +70,6 @@ Definition RCon : list int := map (fun i => Int.shl i (Int.repr 24)) [
   (* 0x40000000 *) (Int.repr 64)
 ].
 
-Definition if_less_than_8{T: Type}(i: nat)(thenF: Z -> T)(elseF: nat -> nat -> Z -> T): T :=
-  match i with
-  | S i_minus_1 => match i_minus_1 with
-    | S (S (S (S (S (S (S i_minus_8)))))) => elseF i_minus_8 i_minus_1 (Z.of_nat i)
-    | _ => thenF (Z.of_nat i)
-    end
-  | _ => thenF (Z.of_nat i)
-  end.
-
-Fixpoint KeyExpansionWord_test(i: nat)(key: list int): int :=
-  if_less_than_8 i
-  (fun i => (Znth i key Int.zero))
-  (fun i_minus_8 i_minus_1 i =>
-    let temp := KeyExpansionWord_test i_minus_1 key in
-    Int.xor temp (KeyExpansionWord_test i_minus_8 key)).
-
-Fixpoint loop_1_8{T: Type}(i: nat)(funLt8: Z -> T)(funGt8: Z -> T -> T -> T): T :=
-  match i with
-  | S i_minus_1 => match i_minus_1 with
-    | S (S (S (S (S (S (S i_minus_8)))))) =>
-      funGt8 (Z.of_nat i) (loop_1_8 i_minus_1 funLt8 funGt8) (loop_1_8 i_minus_8 funLt8 funGt8)
-    | _ => funLt8 (Z.of_nat i)
-    end
-  | _ => funLt8 (Z.of_nat i)
-  end.
-
-Fixpoint construct_list{T: Type}(size: nat)(f: Z -> list T -> T): list T :=
-  match size with
-  | O => []
-  | S n => let prevs := (construct_list n f) in prevs ++ [f (Z.of_nat n) prevs]
-  end.
-
-Definition KeyExpansion1(key: list int): list int := construct_list (Z.to_nat (Nb*(Nr+1)))
-  (fun (i: Z) (w: list int) =>
-    if (i <? 8) then
-      (Znth i key Int.zero)
-    else
-      let temp := (Znth (i-1) w Int.zero) in
-      let temp' := if (i mod Nk =? 0) then
-        Int.xor (SubWord (RotWord temp)) (Znth (i/Nk) RCon Int.zero)
-      else if (i mod Nk =? 4) then
-        SubWord temp
-      else
-        temp
-      in
-        Int.xor (Znth (i-8) w Int.zero) temp').
-
-Fixpoint grow_list{T: Type}(l: list T)(toAdd: nat)(f: Z -> list T -> T): list T :=
-  match toAdd with
-  | O => l
-  | S n => let prevs := (construct_list n f) in prevs ++ [f (Zlength l + Z.of_nat n) prevs]
-  end.
-
-(*Require Import Coq.Program.Basics. for compose *)
-
-(*
-Fixpoint funPow{T: Type}(f: T -> T)(n: nat): T -> T := match n with
-| O => id
-| S m => fun x : T => f ((funPow f m) x)
-end.
-*)
-
-(* takes forever to check:
-Fixpoint KeyExpansionWord(i: nat)(key: list int){struct i}: int :=
-  if_less_than_8 i
-  (fun i => (Znth i key Int.zero))
-  (fun i_minus_8 i_minus_1 i =>
-    let temp := KeyExpansionWord i_minus_1 key in
-    let temp' := if (i mod Nk =? 0) then
-      Int.xor (SubWord (RotWord temp)) (Znth (i/Nk) RCon Int.zero)
-    else if (i mod Nk =? 4) then
-      SubWord temp
-    else
-      temp
-    in
-      Int.xor (KeyExpansionWord_test i_minus_8 key) temp').
-*)
-
-(*
-Fixpoint KeyExpansionWord(i: nat)(key: list int): int :=
-  if_less_than_8 i
-  (fun i => (Znth (Z.of_nat i) key Int.zero))
-  (fun i_minus_8 i_minus_1 i =>
-    let temp := KeyExpansionWord i_minus_1 key in
-    Int.xor temp (KeyExpansionWord i_minus_8 key)).
-*)
-
-Fixpoint KeyExpansionWordTest1(inat: nat)(key: list int): int :=
-  let i := Z.of_nat inat in
-  match inat with
-  | S i1nat => match i1nat with
-    | S (S (S (S (S (S (S i8nat)))))) => 
-      let temp := KeyExpansionWordTest1 i1nat key in
-      Int.xor temp (KeyExpansionWordTest1 i8nat key)
-    | _ => (Znth i key Int.zero)
-    end
-  | _ => (Znth i key Int.zero)
-  end.
-
-Program Fixpoint KeyExpansionWord(i: Z)(key: list int){measure (Z.to_nat i)}: int :=
-  if i <? Nk then
-    (Znth i key Int.zero)
-  else
-    let temp := KeyExpansionWord (i-1) key in
-    Int.xor temp (KeyExpansionWord (i-Nk) key).
-Next Obligation.
-Abort.
-
 Definition GrowKeyByOne(w: list int): list int :=
   let i := Zlength w in
   let temp := (Znth (i-1) w Int.zero) in
@@ -197,31 +89,53 @@ end.
 
 Definition KeyExpansion: list int -> list int := pow_fun GrowKeyByOne (Z.to_nat (Nb*(Nr+1))).
 
+(* arr: list of bytes *)
+Definition get_uint32_le (arr: list Z) (i: Z) : int :=
+ (Int.or (Int.or (Int.or
+            (Int.repr (Znth  i    arr 0))
+   (Int.shl (Int.repr (Znth (i+1) arr 0)) (Int.repr  8)))
+   (Int.shl (Int.repr (Znth (i+2) arr 0)) (Int.repr 16)))
+   (Int.shl (Int.repr (Znth (i+3) arr 0)) (Int.repr 24))).
+
+Definition key_bytes_to_key_words(key_bytes: list Z): list int := [
+  get_uint32_le key_bytes 0;
+  get_uint32_le key_bytes 4;
+  get_uint32_le key_bytes 8;
+  get_uint32_le key_bytes 12;
+  get_uint32_le key_bytes 16;
+  get_uint32_le key_bytes 20;
+  get_uint32_le key_bytes 24;
+  get_uint32_le key_bytes 28
+].
+
+(* Note: clightgen turns global variables of type int to pointers to int, to make them addressable,
+   so aes_init_done is a pointer to int, not an int! *)
 Definition key_expansion_spec :=
   DECLARE _mbedtls_aes_setkey_enc
     WITH ctx : val, key : val, ctx_sh : share, key_sh : share, key_chars : list Z,
-         tables : val, init_done : Z
+         tables : val, aes_init_done: val, init_done : Z, ish: share
     PRE [ _ctx OF (tptr t_struct_aesctx), _key OF (tptr tuchar), _keybits OF tuint  ]
-      PROP (writable_share ctx_sh; readable_share key_sh;
+      PROP (writable_share ctx_sh; readable_share key_sh; readable_share ish;
             Zlength key_chars = 32;
             init_done = 1 (*TODO also prove case where init_done=0*))
       LOCAL (temp _ctx ctx; temp _key key; temp _keybits (Vint (Int.repr 256)); 
-             gvar _aes_init_done (Vint (Int.repr init_done));
+             gvar _aes_init_done aes_init_done;
              gvar _tables tables)
       SEP (data_at_ ctx_sh t_struct_aesctx ctx;
            data_at key_sh (tarray tuchar (4*8)) (map Vint (map Int.repr key_chars)) key;
            (*if init_done ?= 1 then tables_initialized tables else tables_uninitialized tables*)
+           data_at ish tint (Vint (Int.repr init_done)) aes_init_done;
            tables_initialized tables)
     POST [  tint ]
       PROP () 
-      LOCAL (temp ret_temp (Vint Int.zero); gvar _aes_init_done (Vint Int.one))
-      SEP (data_at key_sh (tarray tuchar (4*8)) (map Vint [] (*TODO*)) key;
+      LOCAL (temp ret_temp (Vint Int.zero); gvar _aes_init_done aes_init_done)
+      SEP (data_at key_sh (tarray tuchar (4*8)) (map Vint (map Int.repr key_chars)) key;
            data_at ctx_sh t_struct_aesctx 
                    (Vint (Int.repr 8),
                    (Vint (Int.repr (nested_field_offset t_struct_aesctx [StructField _buf])), 
                    (map Vint [] (*TODO*)))) ctx;
-          tables_initialized tables)
-.
+           data_at ish tint (Vint (Int.repr init_done)) aes_init_done;
+           tables_initialized tables).
 
 Definition Gprog : funspecs := ltac:(with_library prog [ key_expansion_spec ]).
 
@@ -244,16 +158,18 @@ Ltac replace_temp name new_value := match goal with
      let E := fresh "E" in assert_PROP (old_value = new_value) as E;
      [ | replace (temp name old_value) with (temp name new_value) by congruence; clear E ]
 end.
+Tactic Notation "replace_temp" constr(name) constr(new_value) :=
+  replace_temp name new_value.
 Tactic Notation "replace_temp" constr(name) constr(new_value) "by" tactic(t) :=
   replace_temp name new_value; [ t | ].
 
-Definition first_loop_inv00 ctx key tables init_done key_chars ctx_sh key_sh i :=
+Definition first_loop_inv00 ctx key tables aes_init_done init_done key_chars ctx_sh key_sh ish i :=
     PROP ( )
     LOCAL (
       temp _RK  (field_address t_struct_aesctx [StructField _buf] ctx);
       temp _t'1 (field_address t_struct_aesctx [StructField _buf] ctx);
       temp _ctx ctx; temp _key key; temp _keybits (Vint (Int.repr 256));
-      gvar _aes_init_done (Vint (Int.repr init_done)); gvar _tables tables)
+      gvar _aes_init_done aes_init_done; gvar _tables tables)
     SEP (
       field_at ctx_sh t_struct_aesctx [StructField _nr] (Vint (Int.repr 14)) ctx;
       field_at ctx_sh t_struct_aesctx [StructField _rk] 
@@ -261,14 +177,16 @@ Definition first_loop_inv00 ctx key tables init_done key_chars ctx_sh key_sh i :
       field_at ctx_sh t_struct_aesctx [StructField _buf]
         (map Vint (map Int.repr (sublist 0 i key_chars)) ++ (repeat Vundef (Z.to_nat (68-i)))) ctx;
       data_at key_sh (tarray tuchar (4 * 8)) (map Vint (map Int.repr key_chars)) key;
+      data_at ish tint (Vint (Int.repr init_done)) aes_init_done;
       tables_initialized tables).
 
-Definition first_loop_inv0 ctx key tables init_done key_chars ctx_sh key_sh :=
-  EX i: Z, first_loop_inv00 ctx key tables init_done key_chars ctx_sh key_sh i.
+Definition first_loop_inv0 ctx key tables aes_init_done init_done key_chars ctx_sh key_sh ish :=
+  EX i: Z, first_loop_inv00 ctx key tables aes_init_done init_done key_chars ctx_sh key_sh ish i.
 
 Lemma body_key_expansion: semax_body Vprog Gprog f_mbedtls_aes_setkey_enc key_expansion_spec.
 Proof.
   start_function.
+  forward.
   match goal with
   | |- semax ?Delta (PROPx ?P1 (LOCALx ?Q1 (SEPx ?R1))) _ _ =>
     forward_if (PROPx P1 (LOCALx Q1 (SEPx R1)))
@@ -279,13 +197,17 @@ Proof.
   (* ctx->nr = 14; *)
   forward.
   (* ctx->rk = RK = ctx->buf; *)
+  forward. replace_temp _t'1 (field_address t_struct_aesctx [StructField _buf] ctx). {
+    entailer!. rewrite field_compatible_field_address by auto with field_compatible. reflexivity.
+  }
   forward. replace_temp _t'1 (field_address t_struct_aesctx [StructField _buf] ctx) by entailer!.
-  forward. replace_temp _RK (field_address t_struct_aesctx [StructField _buf] ctx) by entailer!.
   forward.
   (* first loop: *)
-  forward_for_simple_bound 8 (first_loop_inv0 ctx key tables init_done key_chars ctx_sh key_sh).
+  forward_for_simple_bound 8 
+    (first_loop_inv0 ctx key tables aes_init_done init_done key_chars ctx_sh key_sh ish).
   { (* precondition implies loop invariant: *)
-    entailer!. }
+    entailer!.
+    unfold_field_at 1%nat. entailer!. }
   { (* loop body preserves invariant: *)
     reassoc_seq.
     assert (Int.unsigned (Int.shl (Int.repr i) (Int.repr 2)) = (4 * i)%Z) as E1. {
@@ -306,7 +228,9 @@ Proof.
     assert_PROP ((if field_compatible_dec t_struct_aesctx [StructField _buf] ctx then offset_val 8 ctx
       else Vundef) = field_address t_struct_aesctx [StructField _buf] ctx) by entailer!.
     forward.
-    entailer!. }
+    entailer!.
+    admit.
+  }
   reassoc_seq.
   (* main loop: *)
 
